Qed map_string_marshal_proof

src/program_proof/map_string_marshal_proof.v
@@ -8,16 +8,16 @@ Context `{!heapGS Σ}.
 
 Local Definition encode_maplist (l:list (string * string)) : list u8 :=
   flat_map (λ u,
-              (u64_le (int.Z (length (string_to_bytes u.1)))) ++
+              (u64_le (String.length u.1)) ++
               (string_to_bytes u.1) ++
-              (u64_le (int.Z (length (string_to_bytes u.2)))) ++
+              (u64_le (String.length u.2)) ++
               (string_to_bytes u.2)) l.
 
 Local Lemma encode_maplist_cons k data l :
   encode_maplist ((k, data)::l) =
-              ((u64_le $ int.Z $ length $ string_to_bytes k) ++
+              ((u64_le $ String.length k) ++
                (string_to_bytes k) ++
-               (u64_le $ int.Z $ length $ string_to_bytes data) ++
+               (u64_le $ String.length $ data) ++
                (string_to_bytes data)) ++ encode_maplist l.
 Proof. done. Qed.
 
@@ -51,41 +51,50 @@ Proof.
   wp_apply (wp_WriteInt with "Hs"). iIntros (s') "Hs".
   rewrite replicate_0 /=. wp_store. clear s.
   wp_apply (wp_MapIter_2 _ _ _ _ _
-    (λ kvs_todo kvs_done, ∃ (s : Slice.t) enc,
-      "%Hm" ∷ ⌜kvs_sl = kvs_todo ∪ kvs_done⌝ ∗
-      "%Hdisk" ∷ ⌜dom kvs_todo ## dom kvs_done⌝ ∗
-      "%Henc" ∷ ⌜has_partial_byte_map_encoding enc (size m) (map_zip_with (λ v _, v) m kvs_done)⌝ ∗
+    (λ m_todo m_done, ∃ (s : Slice.t) enc,
+      "%Hm" ∷ ⌜m = m_todo ∪ m_done⌝ ∗
+      "%Hdisk" ∷ ⌜dom m_todo ## dom m_done⌝ ∗
+      "%Henc" ∷ ⌜ has_partial_map_encoding enc (size m) (map_zip_with (λ v _, v) m m_done)⌝ ∗
       "Hl" ∷ l ↦[slice.T byteT] (slice_val s) ∗
       "Hs" ∷ own_slice s byteT 1 enc
-    )%I with "Hkvs_map [Hl Hs]").
+    )%I with "Hmap [Hl Hs]").
   { iExists _, _. iFrame. iPureIntro.
     rewrite right_id_L. split; first done.
-    rewrite /has_partial_byte_map_encoding.
+    rewrite /has_partial_map_encoding.
     split; first set_solver.
     exists [].
     split; first by apply NoDup_nil_2.
     rewrite map_zip_with_empty_r.
     split; first by apply list_to_map_nil.
-    do 2 rewrite -size_dom. rewrite -Hkvs_dom size_dom. done. }
+    rewrite Hmsize. done. }
   { (* core loop *)
-     clear Φ s' mptr. iIntros (k v kvs_todo kvs_done Φ) "!# [HI %Hk] HΦ". iNamed "HI". wp_pures.
-     wp_load. wp_apply (wp_WriteInt with "Hs"). iIntros (s') "Hs". wp_store. clear s.
-     wp_apply wp_slice_len.
-     wp_load. wp_apply (wp_WriteInt with "Hs"). iIntros (s) "Hs". wp_store. clear s'.
-     iSpecialize ("Hkvs_slices" $! k).
-     iMod (readonly_load with "Hkvs_slices") as (q) "Hk".
-     iDestruct (own_slice_small_sz with "Hk") as %Hsz.
-     iEval (rewrite Hm) in "Hk".
-     erewrite lookup_union_Some_l by done. simpl.
-     wp_load. wp_apply (wp_WriteBytes with "[$Hs $Hk]"). iIntros (s') "[Hs _]". wp_store. clear s.
-     iApply "HΦ". iModIntro. iExists _, _. iFrame. iPureIntro.
+     clear Φ s' mptr. iIntros (k v m_todo m_done Φ) "!# [HI %Hk] HΦ". iNamed "HI". wp_pures.
+     wp_load. wp_apply (wp_WriteInt with "Hs"). iIntros (?) "Hs". wp_store. clear s.
+     wp_apply wp_StringToBytes.
+     iIntros (?) "Hksl". iDestruct (own_slice_to_small with "Hksl") as "Hksl".
+     wp_load.
+     wp_apply (wp_WriteBytes with "[$Hs $Hksl]").
+     iIntros (?) "[Hs _]".
+     wp_store.
+     wp_load. wp_apply (wp_WriteInt with "Hs"). iIntros (?) "Hs". wp_store. clear s' s'0.
+     wp_pures.
+     wp_apply wp_StringToBytes.
+     iIntros (?) "Hvsl". iDestruct (own_slice_to_small with "Hvsl") as "Hvsl".
+     wp_load.
+     wp_apply (wp_WriteBytes with "[$Hs $Hvsl]").
+     iIntros (?) "[Hs _]".
+     wp_store.
+     iApply "HΦ".
+     iModIntro.
+     repeat iExists _; iFrame.
+     iPureIntro.
      split.
      { rewrite union_delete_insert //. }
-     assert (kvs_done !! k = None).
+     assert (m_done !! k = None).
      { apply not_elem_of_dom. apply elem_of_dom_2 in Hk. set_solver. }
      split; first set_solver.
      assert (is_Some (m !! k)) as [data Hdata].
-     { apply elem_of_dom. rewrite -Hkvs_dom Hm dom_union. apply elem_of_dom_2 in Hk. set_solver. }
+     { apply elem_of_dom. rewrite Hm dom_union. apply elem_of_dom_2 in Hk. set_solver. }
      destruct Henc as (ls & Hnodup & Hls & Henc). exists (ls ++ [(k, data)]).
      assert (k ∉ ls.*1).
      { intros Hin. eapply (not_elem_of_list_to_map ls). 2:by apply Hin.
@@ -97,19 +106,17 @@ Proof.
      - rewrite list_to_map_snoc //. rewrite Hls.
        change data with ((λ v _, v) data v).
        rewrite map_insert_zip_with. rewrite insert_id //.
-     - rewrite Hdata Henc. cbn. rewrite -!app_assoc. repeat f_equal.
-       rewrite /encode_byte_maplist flat_map_app. f_equal. cbn. rewrite -!app_assoc app_nil_r. repeat f_equal.
-       move:Hsz. rewrite Hdata Hm. erewrite lookup_union_Some_l by done. cbn. intros. word.
+     - subst. cbn. rewrite -!app_assoc. repeat f_equal.
+       rewrite /encode_maplist flat_map_app. f_equal. cbn. rewrite -!app_assoc app_nil_r.
+       rewrite lookup_union in Hdata. rewrite Hk union_Some_l in Hdata.
+       injection Hdata as <-. done.
   }
   iIntros "[Hkvs_map HI]". iNamed "HI".
-  wp_load. iApply "HΦ". iFrame. iSplitL.
-  { iExists _. iFrame. eauto. }
+  wp_load. iApply "HΦ". iFrame.
   iPureIntro. split.
-  - rewrite -size_dom -Hkvs_dom size_dom. rewrite Hmsize. word.
-  - replace m with (map_zip_with (λ (v : list u8) (_ : Slice.t), v) m kvs_sl) at 2. 1:done.
-    clear Henc. rewrite -[map_zip_with _ _ _]map_fmap_id. rewrite map_fmap_zip_with_l; auto.
-    intros k. rewrite -!elem_of_dom. set_solver. *)
-Admitted.
+  - word.
+  - rewrite -[map_zip_with _ _ _]map_fmap_id in Henc. rewrite map_fmap_zip_with_l in Henc; auto.
+Qed.
 
 Lemma wp_DecodeStringMap enc_sl enc enc_rest q m :
   {{{
@@ -123,19 +130,22 @@ Lemma wp_DecodeStringMap enc_sl enc enc_rest q m :
 Proof.
   iIntros "%Φ H HΦ". iNamed "H". wp_call.
   wp_apply wp_ref_to; first by val_ty. iIntros (l) "Hl".
-  (*
-  wp_apply wp_byteMapNew. iIntros (mptr) "Hm".
+  wp_pures. wp_apply wp_ref_of_zero; first done.
+  iIntros (?) "Hnum".
+  wp_pures.
+  wp_apply wp_NewMap. iIntros (mptr) "Hm".
   wp_load.
   destruct Henc as [Hsz (ls & Hnodup & Hls & Henc)]. subst enc.
   rewrite -!app_assoc.
-  wp_apply (wp_ReadInt with "Henc_sl"). iIntros (s') "Hs". wp_store. clear enc_sl.
+  wp_apply (wp_ReadInt with "Henc_sl"). iIntros (s') "Hs". wp_pures.
+  wp_store. wp_store. wp_load.
   wp_apply wp_ref_to; first by val_ty. iIntros (li) "Hli". wp_pures.
-  wp_apply (wp_forUpto (λ i, ∃ s,
-              "Hm" ∷ own_byte_map mptr (list_to_map (take (int.nat i) ls)) ∗
+  wp_apply (wp_forUpto (λ i, ∃ s q,
+              "Hm" ∷ own_map mptr 1 (list_to_map (take (int.nat i) ls)) ∗
               "Hl" ∷ l ↦[slice.T byteT] (slice_val s) ∗
-              "Hs" ∷ own_slice_small s byteT q (encode_byte_maplist (drop (int.nat i) ls) ++ enc_rest)
+              "Hs" ∷ own_slice_small s byteT q (encode_maplist (drop (int.nat i) ls) ++ enc_rest)
   )%I with "[] [$Hli Hm Hl Hs]"); first word.
-  2:{ iExists _. iFrame. }
+  2:{ repeat iExists _. iFrame. }
   { (* core loop *)
     clear s' Φ. iIntros (i Φ) " !#(I & Hli & %Hi) HΦ". iNamed "I". wp_lam.
     replace (int.nat (u64_instance.u64.(word.add) i 1)) with (1 + int.nat i)%nat by word.
@@ -149,31 +159,51 @@ Proof.
     set ls_head := take (int.nat i) ls.
     set ls_tail := drop (1+int.nat i) ls.
     intros Hnodup.
-    rewrite encode_byte_maplist_cons -!app_assoc.
+    rewrite encode_maplist_cons -!app_assoc.
+    wp_apply wp_ref_of_zero; first done.
+    iIntros (?) "?".
+    wp_pures.
+    wp_apply wp_ref_of_zero; first done. iIntros (?) "?".
+    wp_pures.
+    wp_apply wp_ref_of_zero; first done. iIntros (?) "?".
+    wp_pures.
     wp_load.
     wp_apply (wp_ReadInt with "Hs"). iIntros (s') "Hs".
-    wp_apply (wp_ReadInt with "Hs"). iIntros (s'') "Hs".
-    iDestruct (own_slice_small_sz with "Hs") as %Hdatasz.
-    wp_apply (wp_ReadBytesCopy with "Hs").
-    { rewrite !app_length in Hdatasz. word. }
-    iIntros (sl s''') "[Hval Hs]". wp_store. clear s s' s'' Hdatasz.
-    wp_apply (wp_byteMapPut with "[$Hm Hval]").
-    { iDestruct (own_slice_to_small with "Hval") as "$". }
+    wp_pures. wp_store. wp_store.
+    wp_load. wp_load.
+    iDestruct (own_slice_small_sz with "Hs") as %Hsl_sz.
+    wp_apply (wp_ReadBytes with "[$]").
+    { rewrite string_bytes_length. rewrite app_length in Hsl_sz. word. }
+    iIntros "* [Hksl Hs]".
+    wp_pures. wp_store. wp_store. wp_load.
+    wp_apply (wp_ReadInt with "Hs"). iIntros (?) "Hs".
+    wp_pures. wp_store. wp_store.
+    wp_load. wp_load. clear Hsl_sz.
+    iDestruct (own_slice_small_sz with "Hs") as %Hsl_sz.
+    wp_apply (wp_ReadBytes with "[$]").
+    { rewrite string_bytes_length. rewrite app_length in Hsl_sz. word. }
+    iIntros "* [Hvsl Hs]".
+    wp_pures. wp_store. wp_store. wp_load.
+    wp_apply (wp_StringFromBytes with "[$Hvsl]").
+    iIntros "_".
+    wp_load.
+    wp_apply (wp_StringFromBytes with "[$Hksl]").
+    iIntros "_".
+    repeat rewrite string_to_bytes_inj.
+    wp_apply (wp_MapInsert with "[$]").
+    { done. }
     iIntros "Hm". wp_pures. iApply "HΦ". iModIntro.
-    iFrame "Hli". iExists _. iFrame. iExactEq "Hm". rewrite /named. f_equal.
+    iFrame "Hli". repeat iExists _. iFrame. iExactEq "Hm". rewrite /named. f_equal.
     rewrite list_to_map_snoc //.
     rewrite fmap_app NoDup_app in Hnodup.
     destruct Hnodup as (_ & Hnin & _). intros Hin. eapply Hnin; first done.
     eapply elem_of_list_fmap_1_alt.
     - apply elem_of_list_here.
     - done. }
-  iIntros "(I & Hli)". iNamed "I". wp_load. wp_pures. iApply "HΦ". iModIntro.
+  iIntros "(I & Hli)". iNamed "I". wp_pures. iApply "HΦ". iModIntro.
   rewrite take_ge.
   2:{ rewrite -Map.size_list_to_map // Hls. word. }
   rewrite Hls. iFrame "Hm".
-  rewrite drop_ge.
-  2:{ rewrite -Map.size_list_to_map // Hls. word. }
-  done.
-Admitted.
+Qed.
 
 End map_string_marshal_proof.
