external/Goose/github_com/mit_pdos/gokv/map_string_marshal.v
@@ -6,51 +6,13 @@ Section code.
 Context `{ext_ty: ext_types}.
 Local Coercion Var' s: expr := Var s.
 
-Definition EncodeMapStringToBytes: val :=
-  rec: "EncodeMapStringToBytes" "kvs" :=
-    let: "enc" := ref_to (slice.T byteT) (NewSlice byteT #0) in
-    "enc" <-[slice.T byteT] (marshal.WriteInt (![slice.T byteT] "enc") (MapLen "kvs"));;
-    MapIter "kvs" (λ: "k" "v",
-      let: "kb" := StringToBytes "k" in
-      "enc" <-[slice.T byteT] (marshal.WriteInt (![slice.T byteT] "enc") (slice.len "kb"));;
-      "enc" <-[slice.T byteT] (marshal.WriteBytes (![slice.T byteT] "enc") "kb");;
-      "enc" <-[slice.T byteT] (marshal.WriteInt (![slice.T byteT] "enc") (slice.len "v"));;
-      "enc" <-[slice.T byteT] (marshal.WriteBytes (![slice.T byteT] "enc") "v"));;
-    ![slice.T byteT] "enc".
-
-Definition DecodeMapStringToBytes: val :=
-  rec: "DecodeMapStringToBytes" "enc_in" :=
-    let: "enc" := ref_to (slice.T byteT) "enc_in" in
-    let: "kvs" := NewMap stringT (slice.T byteT) #() in
-    let: ("numEntries", "enc") := marshal.ReadInt (![slice.T byteT] "enc") in
-    let: "i" := ref_to uint64T #0 in
-    (for: (λ: <>, (![uint64T] "i") < "numEntries"); (λ: <>, "i" <-[uint64T] ((![uint64T] "i") + #1)) := λ: <>,
-      let: "keyLen" := ref (zero_val uint64T) in
-      let: ("0_ret", "1_ret") := marshal.ReadInt (![slice.T byteT] "enc") in
-      "keyLen" <-[uint64T] "0_ret";;
-      "enc" <-[slice.T byteT] "1_ret";;
-      let: "key" := NewSlice byteT (![uint64T] "keyLen") in
-      SliceCopy byteT "key" (SliceTake (![slice.T byteT] "enc") (![uint64T] "keyLen"));;
-      "enc" <-[slice.T byteT] (SliceSkip byteT (![slice.T byteT] "enc") (![uint64T] "keyLen"));;
-      let: "valLen" := ref (zero_val uint64T) in
-      let: ("0_ret", "1_ret") := marshal.ReadInt (![slice.T byteT] "enc") in
-      "valLen" <-[uint64T] "0_ret";;
-      "enc" <-[slice.T byteT] "1_ret";;
-      let: "val" := NewSlice byteT (![uint64T] "valLen") in
-      SliceCopy byteT "val" (SliceTake (![slice.T byteT] "enc") (![uint64T] "valLen"));;
-      "enc" <-[slice.T byteT] (SliceSkip byteT (![slice.T byteT] "enc") (![uint64T] "valLen"));;
-      MapInsert "kvs" (StringFromBytes "key") "val";;
-      Continue);;
-    "kvs".
-
 Definition EncodeStringMap: val :=
   rec: "EncodeStringMap" "kvs" :=
     let: "enc" := ref_to (slice.T byteT) (NewSlice byteT #0) in
     "enc" <-[slice.T byteT] (marshal.WriteInt (![slice.T byteT] "enc") (MapLen "kvs"));;
     MapIter "kvs" (λ: "k" "v",
-      let: "kb" := StringToBytes "k" in
-      "enc" <-[slice.T byteT] (marshal.WriteInt (![slice.T byteT] "enc") (slice.len "kb"));;
-      "enc" <-[slice.T byteT] (marshal.WriteBytes (![slice.T byteT] "enc") "kb");;
+      "enc" <-[slice.T byteT] (marshal.WriteInt (![slice.T byteT] "enc") (StringLength "k"));;
+      "enc" <-[slice.T byteT] (marshal.WriteBytes (![slice.T byteT] "enc") (StringToBytes "k"));;
       "enc" <-[slice.T byteT] (marshal.WriteInt (![slice.T byteT] "enc") (StringLength "v"));;
       "enc" <-[slice.T byteT] (marshal.WriteBytes (![slice.T byteT] "enc") (StringToBytes "v")));;
     ![slice.T byteT] "enc".
@@ -58,25 +20,30 @@ Definition EncodeStringMap: val :=
 Definition DecodeStringMap: val :=
   rec: "DecodeStringMap" "enc_in" :=
     let: "enc" := ref_to (slice.T byteT) "enc_in" in
+    let: "numEntries" := ref (zero_val uint64T) in
     let: "kvs" := NewMap stringT stringT #() in
-    let: ("numEntries", "enc") := marshal.ReadInt (![slice.T byteT] "enc") in
+    let: ("0_ret", "1_ret") := marshal.ReadInt (![slice.T byteT] "enc") in
+    "numEntries" <-[uint64T] "0_ret";;
+    "enc" <-[slice.T byteT] "1_ret";;
+    let: "numEntries2" := ![uint64T] "numEntries" in
     let: "i" := ref_to uint64T #0 in
-    (for: (λ: <>, (![uint64T] "i") < "numEntries"); (λ: <>, "i" <-[uint64T] ((![uint64T] "i") + #1)) := λ: <>,
-      let: "keyLen" := ref (zero_val uint64T) in
+    (for: (λ: <>, (![uint64T] "i") < "numEntries2"); (λ: <>, "i" <-[uint64T] ((![uint64T] "i") + #1)) := λ: <>,
+      let: "ln" := ref (zero_val uint64T) in
+      let: "key" := ref (zero_val (slice.T byteT)) in
+      let: "val" := ref (zero_val (slice.T byteT)) in
       let: ("0_ret", "1_ret") := marshal.ReadInt (![slice.T byteT] "enc") in
-      "keyLen" <-[uint64T] "0_ret";;
+      "ln" <-[uint64T] "0_ret";;
       "enc" <-[slice.T byteT] "1_ret";;
-      let: "key" := NewSlice byteT (![uint64T] "keyLen") in
-      SliceCopy byteT "key" (SliceTake (![slice.T byteT] "enc") (![uint64T] "keyLen"));;
-      "enc" <-[slice.T byteT] (SliceSkip byteT (![slice.T byteT] "enc") (![uint64T] "keyLen"));;
-      let: "valLen" := ref (zero_val uint64T) in
+      let: ("0_ret", "1_ret") := marshal.ReadBytes (![slice.T byteT] "enc") (![uint64T] "ln") in
+      "key" <-[slice.T byteT] "0_ret";;
+      "enc" <-[slice.T byteT] "1_ret";;
       let: ("0_ret", "1_ret") := marshal.ReadInt (![slice.T byteT] "enc") in
-      "valLen" <-[uint64T] "0_ret";;
+      "ln" <-[uint64T] "0_ret";;
       "enc" <-[slice.T byteT] "1_ret";;
-      let: "val" := NewSlice byteT (![uint64T] "valLen") in
-      SliceCopy byteT "val" (SliceTake (![slice.T byteT] "enc") (![uint64T] "valLen"));;
-      "enc" <-[slice.T byteT] (SliceSkip byteT (![slice.T byteT] "enc") (![uint64T] "valLen"));;
-      MapInsert "kvs" (StringFromBytes "key") (StringFromBytes "val");;
+      let: ("0_ret", "1_ret") := marshal.ReadBytes (![slice.T byteT] "enc") (![uint64T] "ln") in
+      "val" <-[slice.T byteT] "0_ret";;
+      "enc" <-[slice.T byteT] "1_ret";;
+      MapInsert "kvs" (StringFromBytes (![slice.T byteT] "key")) (StringFromBytes (![slice.T byteT] "val"));;
       Continue);;
     "kvs".
 
